reformulated the semantic proof obligations to use a form of Temporal Logic (similar to TLA)

unity/models/det.lean
@@ -24,8 +24,45 @@ def prog.take_step (s : prog lbl α) : option lbl → α → α
   | none := id
   | (some e) := s^.step e
 
+def prog.action_of (s : prog lbl α) (e : option lbl) (σ σ' : α) : Prop :=
+s^.take_step e σ = σ'
+
+def is_step (s : prog lbl α) (σ σ' : α) : Prop :=
+∃ ev, prog.action_of s ev σ σ'
+
+def prog.falsify (s : prog lbl α) (ev : option lbl) (p : pred α) : Prop
+:= ∀ σ, p σ → ¬ (p (s^.take_step ev σ))
+
 def prog.transient (s : prog lbl α) (p : pred α) : Prop
-:= ∃ ev, ∀ σ, p σ → ¬ (p (s^.take_step ev σ))
+:= ∃ ev, prog.falsify s ev p
+
+def prog.falsify_action (s : prog lbl α) (p : pred α) (ev : option lbl)
+  (h : s.falsify ev p)
+: •p ⟹ ( ⟦ prog.action_of s ev ⟧ ⟶ ⟦ λ _, ~ p ⟧ ) :=
+begin
+  unfold prog.transient at h,
+  intros τ H₀ H₁,
+  unfold temporal.action prog.action_of at H₁,
+  unfold temporal.action,
+  rw -H₁,
+  apply h,
+  apply H₀
+end
+
+lemma prog.falsify.negate
+   {s : prog lbl α} {act : option lbl} {p : pred' α}
+:  prog.falsify s act p
+→  •p && ⟦ s^.action_of act ⟧ ⟹ <>~•p :=
+begin
+  intros FALSE τ H,
+  assert GOAL : ⟦ λ _, ~ p ⟧ τ,
+  { cases H with H₀ H₁,
+    apply prog.falsify_action s p act FALSE
+    ; assumption },
+  unfold temporal.eventually,
+  existsi 1,
+  apply GOAL
+end
 
 lemma prog.transient_false (s : prog lbl α) : prog.transient s False :=
 begin
@@ -49,9 +86,6 @@ begin
   apply h _ h₂
 end
 
-def is_step (s : prog lbl α) (σ σ' : α) : Prop :=
-∃ e, s^.take_step e σ = σ'
-
 instance prog_is_system : unity.system (prog lbl α) :=
   { σ := α
   , init := prog.init
@@ -61,14 +95,15 @@ instance prog_is_system : unity.system (prog lbl α) :=
   , transient_str := prog.transient_str
   }
 
-open nat
+open temporal
 
 structure ex (p : prog lbl α) (τ : stream α) : Prop :=
     (init : τ 0 = p^.first)
     (safety : ∀ i, ∃ e, p^.take_step e (τ i) = τ (i+1))
-    (liveness : ∀ i e, ∃ j, p^.take_step e (τ (i+j)) = τ (i+j+1))
+    (liveness : ∀ e, ([] <> ⟦ p.action_of e ⟧) τ)
 
 open unity
+open nat
 
 def run (s : prog lbl α) (τ : stream (option lbl)) : stream α
   | 0 := prog.first s
@@ -93,11 +128,15 @@ lemma ex_fin_sched [finite lbl] (s : prog lbl α) : ex s (run s fin_sched) :=
   , safety := take i, ⟨fin_sched i,rfl⟩
   , liveness :=
     begin
-      intros i e,
+      intros e i,
       cases inf_repeat_fin_inter ((pos_finite.to_nat $ option lbl)^.f e) i with j h,
+      unfold eventually,
       existsi j, unfold fin_sched,
+      simp [stream.drop_drop],
+      unfold action prog.action_of stream.drop,
       simp [add_one_eq_succ],
-      apply congr, rw [stream.map_app,h,bijection.f_inv],
+      apply congr,
+      { rw [stream.map_app,h,bijection.f_inv] },
       refl
     end }
 
@@ -106,12 +145,16 @@ lemma ex_inf_sched [infinite lbl] (s : prog lbl α) : ex s (run s inf_sched) :=
   , safety := take i, ⟨inf_sched i,rfl⟩
   , liveness :=
     begin
-      intros i e,
+      intros e i,
       cases inf_repeat_inf_inter ((infinite.to_nat $ option lbl)^.f e) i with j h,
+      unfold eventually,
       existsi j, unfold fin_sched,
+      simp [stream.drop_drop],
+      unfold action prog.action_of stream.drop,
       simp [add_one_eq_succ],
-      apply congr, apply congr_arg,
-      unfold inf_sched, rw [stream.map_app,h,bijection.f_inv],
+      apply congr,
+      { apply congr_arg,
+        unfold inf_sched, rw [stream.map_app,h,bijection.f_inv] },
       refl
     end }
 
@@ -129,19 +172,17 @@ include T₀
 variables (τ : stream α)
 
 lemma transient.semantics (h : ex s τ)
-: ∀ (i : ℕ), p (τ i) → (∃ (j : ℕ), ¬p (τ (i + j))) :=
+: ([]<>~•p) τ :=
 begin
-  intros i hp,
   unfold prog.transient at T₀,
   cases T₀ with ev T₀,
-  note sch := h.liveness i ev,
-  cases sch with j sch,
-  cases classical.em (p (τ (i + j))) with h h,
-  { existsi j + 1,
-    rw [-add_assoc,-sch],
-    apply T₀ _ h, },
-  { existsi j,
-    apply h }
+  cases temporal.em' (• p) τ with hp hnp,
+  { note occ := coincidence hp (h.liveness ev),
+    rw -eventually_eventually,
+    apply hence_map _ _ occ,
+    apply ex_map,
+    apply T₀.negate },
+  { apply hnp }
 end
 
 end soundness
