unity/predicate.lean
@@ -2,55 +2,66 @@
 
 namespace predicate
 
+universe variable u
+
+variables {α β : Type u}
+
 def pred' α := α → Prop
 
-def False {α} : pred' α := λ_, false
-def True {α} : pred' α := λ_, true
+def False : pred' α := λ_, false
+def True : pred' α := λ_, true
 
 @[reducible]
-def p_or {α} (p₀ p₁ : pred' α) : pred' α
+def p_or (p₀ p₁ : pred' α) : pred' α
 := λx, p₀ x ∨ p₁ x
 
 @[reducible]
-def p_and {α} (p₀ p₁ : pred' α) : pred' α
+def p_and (p₀ p₁ : pred' α) : pred' α
 := λx, p₀ x ∧ p₁ x
 
-def p_impl {α} (p₀ p₁ : pred' α) : pred' α
+def p_impl (p₀ p₁ : pred' α) : pred' α
 := λx, p₀ x → p₁ x
 
-def p_entails {α} (p₀ p₁ : pred' α) : Prop
+def p_entails (p₀ p₁ : pred' α) : Prop
 := ∀ x, p₀ x → p₁ x
 
 @[reducible]
-def p_not {α} (p : pred' α) : pred' α
+def p_not (p : pred' α) : pred' α
 := λx, ¬ p x
 
 @[simp]
-lemma False_eq_false {β} (τ : β) : False τ = false := rfl
+lemma False_eq_false (τ : β) : False τ = false := rfl
 @[simp]
-lemma True_eq_true {β} (τ : β) : True τ = true := rfl
+lemma True_eq_true (τ : β) : True τ = true := rfl
+
+def ew (p : β → Prop) : Prop :=
+∀ x, p x
 
 infixl ` || ` := p_or
 infixl ` && ` := p_and
 infixl ` ⟶ `:60 := p_impl
 infix ` ⟹ `:60 := p_entails
+notation `⦃ `:max act ` ⦄` := ew act
 
 notation `~`:75 x := p_not x
 
-lemma p_imp_p_imp_p_imp {α} {p p' q q' : pred' α} {τ}
+lemma p_imp_p_imp_p_imp {p p' q q' : pred' α} {τ}
   (hp : (p' ⟶ p) τ)
   (hq : (q ⟶ q') τ)
 : ( p ⟶ q ) τ → ( p' ⟶ q' ) τ :=
 take hpq, hq ∘ hpq ∘ hp
 
-lemma p_imp_p_imp_p_imp_left {α} {p p' q : pred' α} {τ}
+lemma p_imp_p_imp_p_imp_left {p p' q : pred' α} {τ}
   (hp : (p' ⟶ p) τ)
 : ( p ⟶ q ) τ → ( p' ⟶ q ) τ :=
 p_imp_p_imp_p_imp hp id
 
-lemma p_imp_p_imp_p_imp_right {α} {p q q' : pred' α} {τ}
+lemma p_imp_p_imp_p_imp_right {p q q' : pred' α} {τ}
   (hq : (q ⟶ q') τ)
 : ( p ⟶ q ) τ → ( p ⟶ q' ) τ :=
 p_imp_p_imp_p_imp id hq
+
+lemma p_not_eq_not (p : pred' β) (τ) : ¬ p τ ↔ (~p) τ :=
+by refl
 
 end predicate
